tried a first version of "predictor validity".  It's not strong enough. in addition to saying that (predictor fuel) is finite for each fuel, we also need to say that there's a large enough F s.t. (predictor F) = (predictor fuel) for all fuel >= F.
To prove this (about the F), we need to bound the fuel required for the
spilled trace in terms of only the source trace and the source program -
that is, without referencing any proof about the source program.  This is
necessary, since any proof about the source program would depend on
the starting memory and trace of the program, and we need F to be
independent of these.

I'm not totally convinced by that argument, so I'll try again.  Look at
the lemma 'last_step' in Pipeline.v.  That's the sort of thing we need -
that the amount of fuel required for the predictor function is dependent
only on the predictor function.  It can't be dependent on a hypothesis of
the form 'FlatToRiscvCommon.runsto initial post', as in runsTo_sane, since
we need some assumptions about the starting trace and memory to get to this
hypothesis.  So, as mentioned above, we really do need to bound the fuel
required only in terms of the source trace and the source program.
This makes a lot of sense - we've gone to so much effort to show that the
target-level predictor function depends only on the source trace and
source program, it only makes sense that we'd need to prove the same thing
about the amount of fuel we need to give to the target predictor function.

Of course, this whole issue goes away if we use excluded middle.

compiler/src/compiler/FlatToRiscvDef.v
@@ -543,6 +543,28 @@ Section FlatToRiscv1.
     | nil, _ => predict_rest t
     end.
 
+    Inductive predictorLE_valid : (list LeakageEvent -> option qLeakageEvent) -> Prop :=
+    | validLE_nil_end :
+      forall f, f [] = Some qendLE ->
+                predictorLE_valid f
+    | validLE_nil_none :
+      forall f, f [] = None ->
+                predictorLE_valid f
+    | validLE_cons :
+      forall f e, f [] = Some (quotLE e) ->
+                  predictorLE_valid (fun t => f (e :: t)) ->
+                  predictorLE_valid f.
+    Notation predictor_valid := Semantics.predictor_valid.
+
+    Lemma predictLE_with_prefix_valid k f :
+      predictorLE_valid f ->
+      predictorLE_valid (predictLE_with_prefix k f).
+    Proof.
+      intros. induction k.
+      - assumption.
+      - eapply validLE_cons; [reflexivity|]. assumption.
+    Qed.
+    
     Definition rnext_fun' rnext_stmt (fuel : nat) (next : trace -> option qevent) (t_so_far : trace)
       (mypos : Z)
       (sp_val : word) (params rets : list Z) fbody (rt_so_far : list LeakageEvent)
@@ -577,6 +599,17 @@ Section FlatToRiscv1.
                               (f t_so_far')
                               rt_so_far''))
                     rt_so_far.
+
+    Lemma rnext_fun'_preserves_valid rnext_stmt (fuel : nat) next k mypos sp_val params rets fbody f :
+      (forall k, predictorLE_valid (f k)) ->
+      (forall k' mypos' sp_val' offset fbody f',
+          (forall k, predictorLE_valid (f' k)) ->
+          predictorLE_valid (fun rk' => rnext_stmt fuel next k' mypos' sp_val' offset fbody rk' f')) ->
+      predictorLE_valid (fun rk => rnext_fun' rnext_stmt fuel next k mypos sp_val params rets fbody rk f).
+    Proof.
+      intros. cbv [rnext_fun']. apply predictLE_with_prefix_valid. apply H0. intros.
+      apply predictLE_with_prefix_valid. auto.
+    Qed.      
 
     Check (match 5%nat with | S _ | O => 5%nat end).
 
@@ -732,7 +765,68 @@ Section FlatToRiscv1.
           end
       end.
 
+    Lemma rnext_stmt_preserves_valid next k mypos sp_val offset fbody f :
+      (*predictor_valid next ->*)
+      (forall k, predictorLE_valid (f k)) ->
+      forall fuel,
+        predictorLE_valid (fun rk' => rnext_stmt fuel next k mypos sp_val offset fbody rk' f).
+    Proof.
+      intros. generalize dependent f. revert fbody. revert offset. revert sp_val. revert mypos. revert k.
+      induction fuel.
+      - intros. simpl. apply validLE_nil_none. reflexivity.
+      - intros. destruct fbody; cbn [rnext_stmt].
+        + destruct (next k) as [q|]; try (apply validLE_nil_none; reflexivity).
+          destruct q; try (apply validLE_nil_none; reflexivity).
+          apply predictLE_with_prefix_valid. auto.
+        + destruct (next k) as [q|]; try (apply validLE_nil_none; reflexivity).
+          destruct q; try (apply validLE_nil_none; reflexivity).
+          apply predictLE_with_prefix_valid. auto.
+        + destruct (next k) as [q|]; try (apply validLE_nil_none; reflexivity).
+          destruct q; try (apply validLE_nil_none; reflexivity).
+          apply predictLE_with_prefix_valid. auto.
+        + apply predictLE_with_prefix_valid. apply IHfuel. auto.
+        + apply predictLE_with_prefix_valid. auto.
+        + destruct op. all: try destruct (leak_op _ _ _ _); try (apply validLE_nil_none; reflexivity).
+          all: try apply predictLE_with_prefix_valid. all: auto.
+          all: destruct (next k) as [q|]; try (apply validLE_nil_none; reflexivity).
+          all: try destruct q; try (apply validLE_nil_none; reflexivity).
+          all: try destruct (leak_op _ _ _ _); try (apply validLE_nil_none; reflexivity).
+          all: try apply predictLE_with_prefix_valid. all: auto.
+          all: destruct (next (_ ++ _)) as [q|]; try (apply validLE_nil_none; reflexivity).
+          all: destruct q; try (apply validLE_nil_none; reflexivity).
+          all: destruct (leak_op _ _ _ _); try (apply validLE_nil_none; reflexivity).
+          all: apply predictLE_with_prefix_valid. all: auto.
+        + apply predictLE_with_prefix_valid. auto.
+        + destruct (next k) as [q|]; try (apply validLE_nil_none; reflexivity).
+          destruct q; try (apply validLE_nil_none; reflexivity).
+          apply predictLE_with_prefix_valid. apply IHfuel. intros.
+          apply predictLE_with_prefix_valid. auto.
+        + apply IHfuel. intros. destruct (next _) as [q|]; try (apply validLE_nil_none; reflexivity).
+          destruct q; try (apply validLE_nil_none; reflexivity).
+          destruct b.
+          -- apply predictLE_with_prefix_valid. apply IHfuel. intros.
+             apply predictLE_with_prefix_valid. apply IHfuel. auto.
+          -- apply predictLE_with_prefix_valid. auto.
+        + auto.
+        + auto.
+        + destruct (map.get e_env f0).
+          -- destruct p. destruct p. destruct (map.get e f0).
+             ++ apply predictLE_with_prefix_valid. apply rnext_fun'_preserves_valid; assumption.
+             ++ apply validLE_nil_none. reflexivity.
+          -- apply validLE_nil_none. reflexivity.
+        + apply predictLE_with_prefix_valid. auto.
+    Qed.      
+
     Definition rnext_fun := rnext_fun' rnext_stmt.
+    Check rnext_fun'_preserves_valid.
+    Lemma rnext_fun_valid fuel next k mypos sp_val params rets fbody f :
+      (forall k', predictorLE_valid (f k')) ->
+      predictorLE_valid (fun rk => rnext_fun fuel next k mypos sp_val params rets fbody rk f).
+    Proof.
+      cbv [rnext_fun]. intros. apply rnext_fun'_preserves_valid.
+      - auto.
+      - intros. apply rnext_stmt_preserves_valid. auto.
+    Qed.       
   End WithOtherEnv.
   End WithEnv.
 
